

$$\textcircled{2} \quad \|\vec{x}\|^2 + \|\vec{y}\|^2 = \frac{1}{2} (\|\vec{x} + \vec{y}\|^2 + \|\vec{x} - \vec{y}\|^2)$$

$$\frac{1}{2} (\|\vec{x} + \vec{y}\|^2 + \|\vec{x} - \vec{y}\|^2) = \frac{1}{2} (\langle \vec{x} + \vec{y}, \vec{x} + \vec{y} \rangle + \langle \vec{x} - \vec{y}, \vec{x} - \vec{y} \rangle) =$$

$$= \frac{1}{2} (\langle \vec{x} + \vec{y}, \vec{x} + \vec{y} \rangle + \langle \vec{x} - \vec{y}, \vec{x} - \vec{y} \rangle)$$

$$= \frac{1}{2} (\langle \vec{x}, \vec{x} + \vec{y} \rangle + \langle \vec{y}, \vec{x} + \vec{y} \rangle + \langle \vec{x}, \vec{x} - \vec{y} \rangle - \langle \vec{y}, \vec{x} - \vec{y} \rangle) =$$

$$= \frac{1}{2} (\langle \vec{x}, \vec{x} \rangle + \langle \vec{x}, \vec{y} \rangle + \langle \vec{y}, \vec{x} \rangle + \langle \vec{y}, \vec{y} \rangle +$$

$$+ \langle \vec{x}, \vec{x} \rangle - \langle \vec{x}, \vec{y} \rangle - \langle \vec{y}, \vec{x} \rangle + \langle \vec{y}, \vec{y} \rangle) =$$

$$= \frac{1}{2} (2\langle \vec{x}, \vec{x} \rangle + 2\langle \vec{y}, \vec{y} \rangle) = \langle \vec{x}, \vec{x} \rangle + \langle \vec{y}, \vec{y} \rangle = \|\vec{x}\|^2 + \|\vec{y}\|^2$$